\documentclass[11pt]{article}
\usepackage{graphicx}
\usepackage{amssymb}
\usepackage{epstopdf}
\DeclareGraphicsRule{.tif}{png}{.png}{`convert #1 `dirname #1`/`basename #1 .tif`.png}

\textwidth = 6.5 in
\textheight = 9 in
\oddsidemargin = 0.0 in
\evensidemargin = 0.0 in
\topmargin = 0.0 in
\headheight = 0.0 in
\headsep = 0.0 in
\parskip = 0.2in
\parindent = 0.0in

\newtheorem{theorem}{Theorem}
\newtheorem{corollary}[theorem]{Corollary}
\newtheorem{definition}{Definition}

\begin{document}

\[
y = w_1 x_1 + w_2 x_2 + \ldots w_m x_m + b = {\bf w}  {\bf x} + b\\
\]

\[
y = w'  ({\bf w}  {\bf x}^T + b) + b' = w'  {\bf w}  {\bf x}^T + w'b + b' = {\bf w}'' {\bf x}^T + b''
\]

\[
\sigma({\bf z})_i = \frac{e^{z_i}}{\sum_{j=1}^k e^{z_j}}
\]

\[
\begin{array}{l}
y^{[1]} = w_1^{[1]} x_1 + w_2^{[1]} x_2 + \ldots w_m^{[1]} x_m + b^{[1]} = {\bf w}^{[1]} {\bf x}^T + b^{[1]}\\
y^{[2]} = w_2^{[2]} x_2 + w_2^{[2]} x_2 + \ldots w_m^{[2]} x_m + b^{[2]} = {\bf w}^{[2]} {\bf x}^T + b^{[2]}\\
y^{[3]} = w_3^{[3]} x_3 + w_3^{[3]} x_3 + \ldots w_m^{[3]} x_m + b^{[3]} = {\bf w}^{[3]} {\bf x}^T + b^{[3]}\\
\end{array}
\]

\[
{\bf y} = W {\bf x}^T + {\bf b}
\]

\[
{\bf w} {\bf x} + b
\]

\[
{\bf x}
\]

\[
X
\]

\[
{\bf x}_1
\]
\[
{\bf x}_2
\]
\[
{\bf x}_n
\]

\[
y_1
\]
\[
y_2
\]
\[
y_n
\]


 \end{document}